dafny-qi.profile
@@ -1,1 +1,8 @@
-Dafny 2.3.0.10506
+/home/rob/projects/verified-betrfs.marshalling/lib/Marshalling/../Base/sequences.i.dfy(321,31): Warning: type parameter A of ghost predicate IsPrefix is declared (==), which is unnecessary because the predicate doesn’t contain any compiled code
+/home/rob/projects/verified-betrfs.marshalling/lib/Marshalling/../Base/sequences.i.dfy(328,31): Warning: type parameter A of ghost predicate IsSuffix is declared (==), which is unnecessary because the predicate doesn’t contain any compiled code
+/home/rob/projects/verified-betrfs.marshalling/lib/Marshalling/../Base/sequences.i.dfy(333,37): Warning: type parameter A of ghost function SeqIndexIterate is declared (==), which is unnecessary because the function doesn’t contain any compiled code
+/home/rob/projects/verified-betrfs.marshalling/lib/Marshalling/../Base/sequences.i.dfy(344,30): Warning: type parameter A of ghost function SeqIndex is declared (==), which is unnecessary because the function doesn’t contain any compiled code
+/home/rob/projects/verified-betrfs.marshalling/lib/Marshalling/../Base/sequences.i.dfy(351,33): Warning: type parameter V of ghost function SeqOfLength is declared (==), which is unnecessary because the function doesn’t contain any compiled code
+/home/rob/projects/verified-betrfs.marshalling/lib/Marshalling/MarshalledAccessors.i.dfy(1111,4): Warning: /!\ No terms found to trigger on.
+Fatal Error: ProverException: Unrecognised prover option: smt.qi.profile=true
+Fatal Error: ProverException: Unrecognised prover option: smt.qi.profile=true
